wip: low-level Merkle tree: memory safety of insertion

examples/low-level/merkletree/MerkleTree.Low.fst
@@ -1,6 +1,7 @@
 module MerkleTree.Low
 
 open FStar.All
+open FStar.Mul
 open LowStar.Modifies
 open LowStar.BufferOps
 
@@ -23,21 +24,93 @@ assume val hash_from_hashes: hash -> hash -> Tot hash
 // This number says that the maximum number of values is (2^32 - 1)
 let max_num_elts_lg = 32
 
-val get_values_alloc_size_lg: 
+/// Allocation by power of two
+
+// TODO: optimize using bit manipulation
+val is_pow2: nat -> Tot bool
+let rec is_pow2 n =
+  if n = 0 then false
+  else if n = 1 then true
+  else (n % 2 = 0 && is_pow2 (n / 2))
+
+val pow2_is_pow2:
+  n:nat ->
+  Lemma (is_pow2 (pow2 n))
+	[SMTPat (is_pow2 (pow2 n))]
+let rec pow2_is_pow2 n =
+  if n = 0 then ()
+  else pow2_is_pow2 (n - 1)
+
+val alloc_sz_lg: 
   nelts:nat{nelts > 0} -> 
   GTot (sz:nat{if sz = 0 
     then nelts <= pow2 sz
     else pow2 (sz - 1) < nelts && nelts <= pow2 sz})
-let rec get_values_alloc_size_lg nelts =
+let rec alloc_sz_lg nelts =
   if nelts = 1 then 0
-  else if nelts % 2 = 0 then 1 + get_values_alloc_size_lg (nelts / 2)
-  else 1 + get_values_alloc_size_lg ((nelts + 1) / 2)
+  else if nelts % 2 = 0 then 1 + alloc_sz_lg (nelts / 2)
+  else 1 + alloc_sz_lg ((nelts + 1) / 2)
+
+val pow2_interval_unique:
+  n:nat -> sz1:nat{sz1 > 0} -> sz2:nat{sz2 > 0} ->
+  Lemma (requires (pow2 (sz1 - 1) < n && n <= pow2 sz1 &&
+		  pow2 (sz2 - 1) < n && n <= pow2 sz2))
+	(ensures (sz1 = sz2))
+let pow2_interval_unique n sz1 sz2 =
+  if sz1 > sz2 
+  then Math.Lemmas.pow2_le_compat (sz1 - 1) sz2
+  else if sz1 < sz2
+  then Math.Lemmas.pow2_le_compat (sz2 - 1) sz1
+  else ()
+
+val alloc_sz_lg_inv:
+  nelts:nat -> sz:nat{sz > 0} ->
+  Lemma (requires (pow2 (sz - 1) < nelts && nelts <= pow2 sz))
+	(ensures (alloc_sz_lg nelts = sz))
+let alloc_sz_lg_inv nelts sz =
+  pow2_interval_unique nelts sz (alloc_sz_lg nelts)
+
+val alloc_sz_lg_pow2:
+  nelts:nat ->
+  Lemma (requires (is_pow2 nelts))
+	(ensures (nelts = pow2 (alloc_sz_lg nelts)))
+let rec alloc_sz_lg_pow2 nelts =
+  if nelts = 1 then ()
+  else if nelts % 2 = 0 then alloc_sz_lg_pow2 (nelts / 2)
+  else ()
+
+val alloc_sz_lg_pow2_inc:
+  nelts:nat ->
+  Lemma (requires (is_pow2 nelts))
+	(ensures (alloc_sz_lg (nelts + 1) = 1 + alloc_sz_lg nelts))
+#set-options "--z3rlimit 10"
+let rec alloc_sz_lg_pow2_inc nelts =
+  if nelts = 1 then ()
+  else if nelts % 2 = 0 then alloc_sz_lg_pow2_inc (nelts / 2)
+  else ()
+
+val alloc_sz_lg_not_pow2_inc:
+  nelts:nat{nelts > 0} ->
+  Lemma (requires (~ (is_pow2 nelts)))
+	(ensures (alloc_sz_lg nelts = 
+       		 alloc_sz_lg (nelts + 1)))
+let alloc_sz_lg_not_pow2_inc nelts =
+  let sz1 = alloc_sz_lg nelts in
+  let sz2 = alloc_sz_lg (nelts + 1) in
+  if sz1 > sz2 
+  then Math.Lemmas.pow2_le_compat (sz1 - 1) sz2
+  else if sz1 < sz2
+  then (Math.Lemmas.pow2_le_compat (sz2 - 1) sz1;
+       assert (nelts = pow2 sz1))
+  else ()
+
+/// Low-level Merkle tree data structure
 
 noeq type merkle_tree =
 | MT: nelts:nat{nelts > 0 && nelts < pow2 max_num_elts_lg} -> 
       // The value buffer will be resized when elements are added.
       // Resizing mechanism will be similar to that of C++ vector.
-      values:elem_buf{B.length values = pow2 (get_values_alloc_size_lg nelts)} ->
+      values:elem_buf{B.length values = pow2 (alloc_sz_lg nelts)} ->
       // The actual number of internal roots should be equal to 
       // the number of "set" bits of `nelts`.
       iroots:hash_buf{B.length iroots = max_num_elts_lg} ->
@@ -67,34 +140,44 @@ val insert_nelts:
 let insert_nelts nelts =
   nelts + 1
 
-// TODO: optimize using bit manipulation
-val is_pow2: nat -> Tot bool
-let rec is_pow2 n =
-  if n = 0 then false
-  else if n = 1 then true
-  else (n % 2 = 0 && is_pow2 (n / 2))
-
-val get_values_alloc_size_lg_eq:
-  nelts:nat{nelts > 0} ->
-  Lemma (requires (~ (is_pow2 nelts)))
-	(ensures (get_values_alloc_size_lg nelts = 
-       		 get_values_alloc_size_lg (nelts + 1)))
-let get_values_alloc_size_lg_eq nelts =
-  admit ()
+// TODO: so inefficient if recursive; maybe it's already defined somewhere?
+val buffer_copy:
+  #a:Type -> l1:nat{l1 > 0} -> b1:B.buffer a{B.length b1 = l1} ->
+  b2:B.buffer a{B.length b2 >= l1} ->
+  HST.ST unit
+	 (requires (fun h0 -> B.live h0 b1 /\ B.live h0 b2 /\ B.disjoint b1 b2))
+	 (ensures (fun h0 _ h1 ->
+	   modifies (loc_buffer b2) h0 h1 /\
+	   B.as_seq h1 b1 == S.slice (B.as_seq h1 b2) 0 l1))
+let rec buffer_copy #a l1 b1 b2 =
+  admit () // Do we have iteration for buffers, or something like `memcpy`?
 
 val insert_values:
   nelts:nat{nelts > 0 && nelts < pow2 max_num_elts_lg - 1} -> 
-  vs:elem_buf{B.length vs = pow2 (get_values_alloc_size_lg nelts)} ->
+  vs:elem_buf{B.length vs = pow2 (alloc_sz_lg nelts)} ->
   elem -> 
-  HST.ST (ivs:elem_buf{B.length ivs = pow2 (get_values_alloc_size_lg (insert_nelts nelts))})
+  HST.ST (ivs:elem_buf{B.length ivs = pow2 (alloc_sz_lg (insert_nelts nelts))})
 	 (requires (fun h0 -> B.live h0 vs))
-	 (ensures (fun h0 nvs h1 -> B.live h1 nvs))
-#set-options "--z3rlimit 10"
+	 (ensures (fun h0 nvs h1 -> B.live h1 nvs)) // TODO: definitely need stronger postconditions
 let insert_values nelts vs e =
-  if is_pow2 nelts then admit ()
-  else (assume (nelts < pow2 (get_values_alloc_size_lg nelts));
+  if is_pow2 nelts 
+  then (// TODO: need a fine-grained control of indexing and allocation
+       assume (2 * nelts <= pow2 (max_num_elts_lg) - 1);
+       
+       let hh0 = HST.get () in
+       let nvs = B.malloc Monotonic.HyperHeap.root elem_init (UInt32.uint_to_t (2 * nelts)) in
+       B.live_unused_in_disjoint hh0 vs nvs;
+       alloc_sz_lg_pow2 nelts;
+       buffer_copy nelts vs nvs;
+
+       B.upd nvs (UInt32.uint_to_t nelts) e;
+
+       // B.free vs; // TODO: `B.free` the previous values buffer
+
+       alloc_sz_lg_pow2_inc nelts; nvs)
+  else (assume (nelts < pow2 (alloc_sz_lg nelts));
        B.upd vs (UInt32.uint_to_t nelts) e;
-       get_values_alloc_size_lg_eq nelts;
+       alloc_sz_lg_not_pow2_inc nelts;
        vs)
 
 val insert_iroots:
